{
     "@context": {
          "rdf": "http://www.w3.org/1999/02/22-rdf-syntax-ns#",
          "rdfs": "http://www.w3.org/2000/01/rdf-schema#",
          "owl": "http://www.w3.org/2002/07/owl#",
          "schema":"http://schema.org/",
          "codemeta": "https://w3id.org/codemeta/",
          "fair4ml": "https://w3id.org/fair4ml/",
          "cr": "http://mlcommons.org/croissant/",
          "CreativeWork":  {"@id": "schema:CreativeWork"},
          "MediaObject":  {"@id": "schema:MediaObject"},
          "ScholarlyArticle":  {"@id": "schema:ScholarlyArticle"},
          "Thing":  {"@id": "schema:Thing"},
          "archivedAt": {"@id": "schema:archivedAt"},
          "author": {"@id": "schema:author"},
          "citation": {"@id": "schema:citation"},
          "codeRepository": {"@id": "schema:codeRepository"},
          "conditionsOfAccess": {"@id": "schema:conditionsOfAccess"},
          "contributor": {"@id": "schema:contributor"},
          "copyrightHolder": {"@id": "schema:copyrightHolder"},
          "dateCreated": {"@id": "schema:dateCreated"},
          "dateModified": {"@id": "schema:dateModified"},
          "datePublished": {"@id": "schema:datePublished"},
          "description": {"@id": "schema:description"},
          "discussionUrl": {"@id": "schema:discussionUrl"},
          "distribution": {"@id": "schema:distribution"},
          "funding": {"@id": "schema:funding"},
          "identifier": {"@id": "schema:identifier"},
          "inLanguage": {"@id": "schema:inLanguage"},
          "isAccessibleForFree": {"@id": "schema:isAccessibleForFree"},
          "keywords": {"@id": "schema:keywords"},
          "license": {"@id": "schema:license"},
          "maintainer": {"@id": "schema:maintainer"},
          "memoryRequirements": {"@id": "schema:memoryRequirements"},
          "name": {"@id": "schema:name"},
          "operatingSystem": {"@id": "schema:operatingSystem"},
          "processorRequirements": {"@id": "schema:processorRequirements"},
          "releaseNotes": {"@id": "schema:releaseNotes"},
          "softwareHelp": {"@id": "schema:softwareHelp"},
          "softwareRequirements": {"@id": "schema:softwareRequirements"},
          "storageRequirements": {"@id": "schema:storageRequirements"},
          "url": {"@id": "schema:url"},
          "version": {"@id": "schema:version"},

          "buildInstructions": {"@id": "codemeta:buildInstructions"},
          "developmentStatus": {"@id": "codemeta:developmentStatus"},
          "issueTracker": {"@id": "codemeta:issueTracker"},
          "readme": {"@id": "codemeta:readme"},
          "referencePublication": {"@id": "codemeta:referencePublication"}
     },
     "@graph": [
          {
               "@id": "https://w3id.org/fair4ml/",
               "name": [
                    "FAIR4ML JSON-LD Context"
               ],
               "version": "0.1.0",
               "url": {
                    "@id": "https://w3id.org/fair4ml/0.1.0"
               },
               "schema:schemaVersion": {
                    "@id": "https://raw.githubusercontent.com/schemaorg/schemaorg/main/data/releases/26.0/schemaorg-all-http.jsonld"
               },
               "license": {
                    "@id": "https://creativecommons.org/publicdomain/zero/1.0/"
               },
               "owl:versionIRI": {
                    "@id": "https://w3id.org/fair4ml/0.1.0"
               },
               "schema:releaseDate": "2024-16-04",
               "schema:codeRepository": {
                    "@id": "https://github.com/RDA-FAIR4ML/FAIR4ML-schema"
               },
               "schema:author":[
                    {
                         "@type": "Person",
                         "schema:name":"Leyla-Jael Castro"
                    },
                    {
                         "@type": "Person",
                         "schema:name":"Daniel Garijo"
                    },
                    {
                         "@type": "Person",
                         "schema:name":"Dietrich Rebholz-Schuhmann"
                    },
                    {
                         "@type": "Person",
                         "schema:name":"Dhwani Solanki"
                    },
                    {
                         "@type": "Person",
                         "schema:name":"Jenifer Tabita Ciuciu-Kiss"
                    },
                    {
                         "@type": "Person",
                         "schema:name":"Dan Katz"
                    },
                    {
                         "@type": "Person",
                         "schema:name":"Lars Eklund"
                    },
                    {
                         "@type": "Person",
                         "schema:name":"Gnana Bharathy"
                    },
                    {
                         "@type": "Organization",
                         "schema:name":"Research Data Alliance FAIR4ML Task Force"
                    }

               ]
          },
          {
               "@id": "fair4ml:MLModel",
               "@type": "rdfs:Class",
               "rdfs:comment": "Class to represent Machine Learning models that can be run for some task (e.g., those available in HuggingFace). A Machine Learning model may have more than one model distribution.",
               "rdfs:label": "Executable Machine Learning Model",
               "rdfs:subClassOf": {
                    "@id": "schema:CreativeWork"
               }
          },
          {
               "@id": "fair4ml:MLModelEvaluation",
               "@type": "rdfs:Class",
               "rdfs:comment": "Class to represent the evaluation of a Machine Learning model.",
               "rdfs:label": "Machine Learning Model Evaluation",
               "rdfs:subClassOf": {
                    "@id": "schema:CreativeWork"
               }
          },
          {
               "@id": "fair4ml:legal",
               "@type": "rdf:Property",
               "rdfs:comment": "Considerations with respect to legal aspects.",
               "rdfs:label": "legal",
               "schema:domainIncludes": {
                    "@id": "fair4ml:MLModel"
               },
               "schema:rangeIncludes": {
                    "@id": "schema:Text"
               }
          },
          {
               "@id": "fair4ml:ethicalSocial",
               "@type": "rdf:Property",
               "rdfs:comment": "Considerations with respect to ethical and social aspects.",
               "rdfs:label": "ethical, social",
               "schema:domainIncludes": {
                    "@id": "fair4ml:MLModel"
               },
               "schema:rangeIncludes": {
                    "@id": "schema:Text"
               }
          },
          {
               "@id": "fair4ml:evaluatedOn",
               "@type": "rdf:Property",
               "rdfs:comment": "Dataset used for evaluating the model. The dataset used for evaluation may not have been part of the train/test/validation (e.g., a benchmark, extrinsic validation).",
               "rdfs:label": "evaluated on",
               "schema:domainIncludes": {
                    "@id": "fair4ml:MLModel"
               },
               "schema:rangeIncludes": 
               {
                    "@id": "cr:Dataset"
               }
          },
          {
               "@id": "fair4ml:hasEvaluation",
               "@type": "rdf:Property",
               "rdfs:comment": "Relationship to point to an evaluation for the model. It may be an evaluation coming from the training process or with a totally unseen dataset used only for evaluation purposes (e.g., a benchmark, extrinsic validation).",
               "rdfs:label": "has evaluation",
               "schema:domainIncludes": {
                    "@id": "fair4ml:MLModel"
               },
               "schema:rangeIncludes": {
                    "@id": "fair4ml:MLModelEvaluation"
               }
          },
          {
               "@id": "fair4ml:fineTunedFrom",
               "@type": "rdf:Property",
               "rdfs:comment": "Relationship to point to the source model used for fine tuning (if this model was fine-tuned from another one).",
               "rdfs:label": "fine-tuned from",
               "schema:domainIncludes": {
                    "@id": "fair4ml:MLModel"
               },
               "schema:rangeIncludes": {
                    "@id": "fair4ml:MLModel"
               }
          },
          {
               "@id": "fair4ml:hasCO2eEmissions",
               "@type": "rdf:Property",
               "rdfs:comment": "Amount of CO2 equivalent emissions produced by training the model. The unit should be included in the field (e.g., 10 tonnes).",
               "rdfs:label": "has CO2e emissions",
               "schema:domainIncludes": {
                    "@id": "fair4ml:MLModel"
               },
               "schema:rangeIncludes": {
                    "@id": "schema:Text"
               }
          },
          {
               "@id": "fair4ml:intendedUse",
               "@type": "rdf:Property",
               "rdfs:comment": "Purpose and intended use stated to enable users to make a decision as to the suitability of this creative work (e.g., lab protocol, machine learning model, software) to their experimental problem or own use case.",
               "rdfs:label": "intended use",
               "schema:domainIncludes": {
                    "@id": "fair4ml:MLModel"
               },
               "schema:rangeIncludes": [{
                    "@id": "schema:Text"
               },
               {
                    "@id": "schema:DefinedTerm"
               },
               {
                    "@id": "schema:URL"
               }]
          },
          {
               "@id": "fair4ml:mlTask",
               "@type": "rdf:Property",
               "rdfs:comment": "ML task addressed by this ML software or model (e.g., binary classification).",
               "rdfs:label": "ml task",
               "schema:domainIncludes": {
                    "@id": "fair4ml:MLModel"
               },
               "schema:rangeIncludes": [{
                    "@id": "schema:Text"
               },
               {
                    "@id": "schema:DefinedTerm"
               }]
          },
          {
               "@id": "fair4ml:modelCategory",
               "@type": "rdf:Property",
               "rdfs:comment": "Category of this ML model (e.g., Supervised, Unsupervised, Semi-supervised, Reinforcement), learning architecture (e.g., CNN, transformer), underlying algorithm (e.g., logistic regression, random forest, LLM).",
               "rdfs:label": "model category",
               "schema:domainIncludes": {
                    "@id": "fair4ml:MLModel"
               },
               "schema:rangeIncludes": [{
                    "@id": "schema:Text"
               },
               {
                    "@id": "schema:DefinedTerm"
               }] 
          },
          {
               "@id": "fair4ml:modelRisksBiasLimitations",
               "@type": "rdf:Property",
               "rdfs:comment": "Description of the risks and biases of the model, in a human-readable manner.",
               "rdfs:label": "model risks bias limitations",
               "schema:domainIncludes": {
                    "@id": "fair4ml:MLModel"
               },
               "schema:rangeIncludes": {
                    "@id": "schema:Text"
               }
          },
          {
               "@id": "fair4ml:sharedBy",
               "@type": "rdf:Property",
               "rdfs:comment": "Person or Organization who shared the model online (e.g., uploading it to HuggingFace).",
               "rdfs:label": "shared by",
               "schema:domainIncludes": {
                    "@id": "fair4ml:MLModel"
               },
               "schema:rangeIncludes": [{
                    "@id": "schema:Person"
               },
               {
                    "@id": "schema:Organization"
               }] 
          },
          {
               "@id": "fair4ml:testedOn",
               "@type": "rdf:Property",
               "rdfs:comment": "Link to the dataset used to test the model (following train/test/validation splits).",
               "rdfs:label": "tested on",
               "schema:domainIncludes": {
                    "@id": "fair4ml:MLModel"
               },
               "schema:rangeIncludes": [{
                    "@id": "schema:Dataset"
               },
               {
                    "@id": "cr:Dataset"
               }]
          },
          {
               "@id": "fair4ml:trainedOn",
               "@type": "rdf:Property",
               "rdfs:comment": "AI-ready dataset (after pre-processing) used for the training and optimization of this ML model.",
               "rdfs:label": "trained on",
               "schema:domainIncludes": {
                    "@id": "fair4ml:MLModel"
               },
               "schema:rangeIncludes": [{
                    "@id": "schema:Dataset"
               },
               {
                    "@id": "cr:Dataset"
               }]
          },
          {
               "@id": "fair4ml:usageInstructions",
               "@type": "rdf:Property",
               "rdfs:comment": "Description of the instructions needed to run the model (e.g., to do inference on a task). Code snippets may be used for illustration.",
               "rdfs:label": "usage instructions",
               "schema:domainIncludes": {
                    "@id": "fair4ml:MLModel"
               },
               "schema:rangeIncludes": {
                    "@id": "schema:Text"
               }
          },
          {
               "@id": "fair4ml:codeSampleSnippet",
               "@type": "rdf:Property",
               "rdfs:comment": "Code snippet with a usage example of the model.",
               "rdfs:label": "code sample snippet",
               "schema:domainIncludes": {
                    "@id": "fair4ml:MLModel"
               },
               "schema:rangeIncludes": {
                    "@id": "schema:Text"
               }
          },
          {
               "@id": "fair4ml:validatedOn",
               "@type": "rdf:Property",
               "rdfs:comment": "Link to the dataset used to validate the model. Typically the training dataset is a separated set from the train/testing set.",
               "rdfs:label": "validated on",
               "schema:domainIncludes": {
                    "@id": "fair4ml:MLModel"
               },
               "schema:rangeIncludes":
               {
                    "@id": "cr:Dataset"
               }
          },
          {
               "@id": "fair4ml:evaluatedMLModel",
               "@type": "rdf:Property",
               "rdfs:comment": "MLModel evaluated with this evaluation. Reverse property: fair4ml:evaluatedWith.",
               "rdfs:label": "evaluated machine learning model",
               "schema:domainIncludes": {
                    "@id": "fair4ml:MLModelEvaluation"
               },
               "schema:rangeIncludes": {
                    "@id": "fair4ml:MLModel"
               }
          },
          {
               "@id": "fair4ml:evaluationDataset",
               "@type": "rdf:Property",
               "rdfs:comment": "Dataset used for the evaluation.",
               "rdfs:label": "evaluation dataset",
               "schema:domainIncludes": {
                    "@id": "fair4ml:MLModelEvaluation"
               },
               "schema:rangeIncludes": {
                    "@id": "cr:Dataset"
               }
          },
          {
               "@id": "fair4ml:evaluationMetrics",
               "@type": "rdf:Property",
               "rdfs:comment": "Description of the metrics used for evaluating the ML model. Example with Text:  [\"Precision: 0.8\", \"Mean: 0.9\"].  Example with PropertyValue:  [{minValue: 0.0, maxValue: 1.0, value: 0.8, measurementTechnique: \"Precision\"} ...]",
               "rdfs:label": "evaluation metrics",
               "schema:domainIncludes": {
                    "@id": "fair4ml:MLModelEvaluation"
               },
               "schema:rangeIncludes": {
                    "@id": "schema:Text"
               }
               
          },
          {
               "@id": "fair4ml:evaluationResults",
               "@type": "rdf:Property",
               "rdfs:comment": "Summary of the results from the evaluation.",
               "rdfs:label": "evaluation results",
               "schema:domainIncludes": {
                    "@id": "fair4ml:MLModelEvaluation"
               },
               "schema:rangeIncludes": [{
                    "@id": "schema:Text"
               },
               {
                    "@id": "schema:PropertyValue"
               }]
          },
          {
               "@id": "fair4ml:evaluationSoftware",
               "@type": "rdf:Property",
               "rdfs:comment": "Code used to performed the evaluation.",
               "rdfs:label": "evaluation software",
               "schema:domainIncludes": {
                    "@id": "fair4ml:MLModelEvaluation"
               },
               "schema:rangeIncludes": {
                    "@id": "schema:SoftwareSourceCode"
               }
          },
          {
               "@id": "fair4ml:extrinsicEvaluation",
               "@type": "rdf:Property",
               "rdfs:comment": "Indicates whether this evaluation is extrinsic, i.e., done with an existing model, outside the model training scope, and with a totally unseen dataset. It could be done by third-parties or by the authors of the model.",
               "rdfs:label": "extrinsic evaluation",
               "schema:domainIncludes": {
                    "@id": "fair4ml:MLModelEvaluation"
               },
               "schema:rangeIncludes": {
                    "@id": "schema:Boolean"
               }
          }
     ]
}
